HittingSetToSetCover/HittingSetToSetCover_simple.dfy
@@ -10,31 +10,16 @@ method HittingSet_to_SetCover_Method(U: set<int>, S: set<set<int>>, k: nat) retu
   ensures counter <= poly(U, S, k)
 {
   counter := 0;
-
   var SS:set<set<set<int>>> := {}; counter := counter + 1;
-  var U' := U; counter := counter + |U|;
-  while (U' != {})
-    decreases |U'|
-    invariant U' <= U
-    invariant SS == (set u | u in (U - U') :: (set s | s in S && u in s))
-    invariant counter <= 1 + |U| + (|U| - |U'|)*(poly_outer_loop(U, S, k) + 1)
-  {
-    counter := counter + 1;
-    U', SS, counter := HittingSet_to_SetCover_outer_loop(U, S, k, U', SS, counter);
-  }
-  counter := counter + 1;
-  identity_substraction_lemma(U, U');
-
+  // Edge case
   var S_contains_empty:bool := {} in S; counter := counter + |S|*|U|;
-
   if (S_contains_empty) {
-    var SS := {}; counter := counter + 1;
     var S' := S; counter := counter + |S|*|U|;
     while (S' != {})
       decreases |S'|
       invariant S' <= S
       invariant SS == (set s | s in (S - S') :: {s})
-      invariant counter <= 2*|S|*|U| + |U|*(poly_outer_loop(U, S, k) + 2) + 3 + (|S| - |S'|)*(poly_edge_case_loop(U, S, k) + 1)
+      invariant counter <= 2*|S|*|U| + 1 + (|S| - |S'|)*(poly_edge_case_loop(U, S, k) + 1)
     {
       counter := counter + 1;
       S', SS, counter := HittingSet_to_SetCover_edge_case_loop(U, S, k, S', SS, counter);
@@ -43,9 +28,21 @@ method HittingSet_to_SetCover_Method(U: set<int>, S: set<set<int>>, k: nat) retu
     identity_substraction_lemma(S, S');
     return (S, SS, 0), counter;
   }
-  else {
-    return (S, SS, k), counter;
+  // Regular case
+  var U' := U; counter := counter + |U|;
+  while (U' != {})
+    decreases |U'|
+    invariant U' <= U
+    invariant SS == (set u | u in (U - U') :: (set s | s in S && u in s))
+    invariant counter <= |S|*|U| + |U| + 1 + (|U| - |U'|)*(poly_outer_loop(U, S, k) + 1)
+  {
+    counter := counter + 1;
+    U', SS, counter := HittingSet_to_SetCover_outer_loop(U, S, k, U', SS, counter);
   }
+  counter := counter + 1;
+  identity_substraction_lemma(U, U');
+  
+  return (S, SS, k), counter;
 }
 
 
@@ -140,7 +137,7 @@ ensures counter <= counter_in + poly_middle_loop(U, S, k)
     s', s_contains_u, counter := HittingSet_to_SetCover_inner_loop(U, S, k, s, s', u, s_contains_u, counter);
   }
   counter := counter + 1;
-  assert counter <= counter_in + poly_aux_3(U, S, k) by {
+  assert counter <= counter_in + poly_aux(U, S, k) by {
     if_smaller_then_less_cardinality(s, U);
     aux_lemma_1(U, S, k, s, s');
   }
@@ -181,7 +178,7 @@ ensures counter == counter_in + poly_inner_loop(U, S, k)
   }
 }
 
-
+/*
 method HittingSet_to_SetCover_S_contains_empty_loop(U:set<int>, S:set<set<int>>, k:nat, S':set<set<int>>, S_contains_empty:bool, ghost counter_in:nat) returns (S'':set<set<int>>, S_contains_empty':bool, ghost counter:nat)
 // Problem requirements
 requires forall s | s in S ::  s <= U
@@ -210,6 +207,7 @@ ensures counter == counter_in + poly_contains_empty_loop(U, S, k)
   }
   counter := counter + 1;
 }
+*/
 
 
 method HittingSet_to_SetCover_edge_case_loop(U:set<int>, S:set<set<int>>, k:nat, S':set<set<int>>, SS:set<set<set<int>>>, ghost counter_in:nat) returns (S'':set<set<int>>, SS':set<set<set<int>>>, ghost counter:nat)
@@ -239,34 +237,7 @@ ensures counter == counter_in + poly_edge_case_loop(U, S, k)
   counter := counter + |S|*|U|;
 }
 
-ghost function poly_aux_1(U: set<int>, S: set<set<int>>, k: nat) : (o:nat)
-  ensures |S|*|U| + |U|*(poly_outer_loop(U, S, k) + 2) + 2 <= o
-{
-  /*calc <= {
-    |S|*|U| + |U|*(poly_outer_loop(U, S, k) + 2) + 2;
-    |U|*(poly_outer_loop(U, S, k) + 2) + |S|*|U| + 2;
-    (|U|*poly_outer_loop(U, S, k) + |U|*2) + |S|*|U| + 2;
-    |U|*poly_outer_loop(U, S, k) + |S|*|U| + 2*|U| + 2;
-    |U|*(3*|S|*|S|*|U| + 2*|S|*|U|*|U| + 4*|S|*|U| + 3*|S| + |U| + 2) + |S|*|U| + 2*|U| + 2;
-    (3*|S|*|S|*|U|*|U| + 2*|S|*|U|*|U|*|U| + 4*|S|*|U|*|U| + 3*|S|*|U| + |U|*|U| + 2*|U|) + |S|*|U| + 2*|U| + 2;
-    (3*|S|*|S|*|U|*|U| + 2*|S|*|U|*|U|*|U| + 4*|S|*|U|*|U| + 3*|S|*|U| + |U|*|U| + 2*|U|) + |S|*|U| + 2*|U| + 2;
-    3*|S|*|S|*|U|*|U| + 2*|S|*|U|*|U|*|U| + 4*|S|*|U|*|U| + 4*|S|*|U| + |U|*|U| + 4*|U| + 2;
-  }*/
-  3*|S|*|S|*|U|*|U| + 2*|S|*|U|*|U|*|U| + 4*|S|*|U|*|U| + 4*|S|*|U| + |U|*|U| + 4*|U| + 2
-}
-ghost function poly_aux_2(U: set<int>, S: set<set<int>>, k: nat) : (o:nat)
-  ensures poly_aux_1(U, S, k) + |S|*(poly_contains_empty_loop(U, S, k) + 1) + |S|*|U| + |S| + 1 <= o
-{
-  /*calc <= {
-    poly_aux_1(U, S, k) + |S|*(poly_contains_empty_loop(U, S, k) + 1) + |S|*|U| + |S| + 1;
-    poly_aux_1(U, S, k) + |S|*(poly_contains_empty_loop(U, S, k) + 1) + |S|*|U| + |S| + 1;
-    (3*|S|*|S|*|U|*|U| + 2*|S|*|U|*|U|*|U| + 4*|S|*|U|*|U| + 4*|S|*|U| + |U|*|U| + 4*|U| + 2) + |S|*(poly_contains_empty_loop(U, S, k) + 1) + |S|*|U| + |S| + 1;
-    (3*|S|*|S|*|U|*|U| + 2*|S|*|U|*|U|*|U| + 4*|S|*|U|*|U| + 4*|S|*|U| + |U|*|U| + 4*|U| + 2) + |S|*|S|*|U| + |S|*|U| + 2*|S| + |S|*|U| + |S| + 1;
-    3*|S|*|S|*|U|*|U| + 2*|S|*|U|*|U|*|U| + |S|*|S|*|U| + 4*|S|*|U|*|U| + 6*|S|*|U| + |U|*|U| + 3*|S| + 4*|U| + 3;
-  }*/
-  3*|S|*|S|*|U|*|U| + 2*|S|*|U|*|U|*|U| + |S|*|S|*|U| + 4*|S|*|U|*|U| + 6*|S|*|U| + |U|*|U| + 3*|S|  + 4*|U|+ 3
-}
-ghost function poly_aux_3(U: set<int>, S: set<set<int>>, k: nat) : (o:nat)
+ghost function poly_aux(U: set<int>, S: set<set<int>>, k: nat) : (o:nat)
 {
   2*|S|*|U| + 2*|U| + (|U|)*(|U| + 2) + 1
 }
@@ -275,7 +246,7 @@ ghost function poly_inner_loop(U: set<int>, S: set<set<int>>, k: nat) : (o:nat)
   |U| + 1
 }
 ghost function poly_middle_loop(U: set<int>, S: set<set<int>>, k: nat) : (o:nat)
-  ensures |S|*|U| + poly_aux_3(U, S, k) <= o
+  ensures |S|*|U| + poly_aux(U, S, k) <= o
 {
   3*|S|*|U| + 2*|U| + |U|*(|U| + 2) + 1
 }
@@ -308,18 +279,22 @@ ghost function poly(U: set<int>, S: set<set<int>>, k: nat) : (o:nat)
 }
 */
 ghost function poly(U: set<int>, S: set<set<int>>, k: nat) : (o:nat)
-  ensures 2*|S|*|U| + |U|*(poly_outer_loop(U, S, k) + 2) + 4 + |S|*(poly_edge_case_loop(U, S, k) + 1) <= o
-  ensures |S|*|U| + |U|*(poly_outer_loop(U, S, k) + 2) + 2 <= o
+  ensures 2*|S|*|U| + 2 + |S|*(poly_edge_case_loop(U, S, k) + 1) <= o
+  ensures |S|*|U| + |U| + 2 + |U|*(poly_outer_loop(U, S, k) + 1) <= o
 {
-  /*calc == {
-    2*|S|*|U| + |U|*(poly_outer_loop(U, S, k) + 2) + 4 + |S|*(poly_edge_case_loop(U, S, k) + 1);
-    2*|S|*|U| + |U|*(poly_outer_loop(U, S, k) + 2) + 4 + |S|*(2*|S|*|U| + 2*|U| + 1);
-    |U|*(poly_outer_loop(U, S, k) + 2) + 2*|S|*|S|*|U| + 4*|S|*|U| + |S| + 4;
-    |U|*(3*|S|*|S|*|U| + 2*|S|*|U|*|U| + 4*|S|*|U| + 3*|S| + |U| + 4) + 2*|S|*|S|*|U| + 4*|S|*|U| + |S| + 4;
-    (3*|S|*|S|*|U|*|U| + 2*|S|*|U|*|U|*|U| + 4*|S|*|U|*|U| + 3*|S|*|U| + |U|*|U| + 4*|U|) + 2*|S|*|S|*|U| + 4*|S|*|U| + |S| + 4;
-    3*|S|*|S|*|U|*|U| + 2*|S|*|U|*|U|*|U| + 2*|S|*|S|*|U| + 4*|S|*|U|*|U| + 7*|S|*|U| + |U|*|U| + |S| + 4*|U| + 4;
-  }*/
-  3*|S|*|S|*|U|*|U| + 2*|S|*|U|*|U|*|U| + 2*|S|*|S|*|U| + 4*|S|*|U|*|U| + 7*|S|*|U| + |U|*|U| + |S| + 4*|U| + 4
+  calc == {
+    |S|*|U| + |U| + 2 + |U|*(poly_outer_loop(U, S, k) + 1);
+    |S|*|U| + |U| + 2 + |U|*(3*|S|*|S|*|U| + 2*|S|*|U|*|U| + 4*|S|*|U| + 3*|S| + |U| + 3);
+    |S|*|U| + |U| + 2 + (3*|S|*|S|*|U|*|U| + 2*|S|*|U|*|U|*|U| + 4*|S|*|U|*|U| + 3*|S|*|U| + |U|*|U| + 3*|U|);
+    3*|S|*|S|*|U|*|U| + 2*|S|*|U|*|U|*|U| + 4*|S|*|U|*|U| + 4*|S|*|U| + |U|*|U| + 4*|U| + 2;
+  }
+  calc == {
+    2*|S|*|U| + 2 + |S|*(poly_edge_case_loop(U, S, k) + 1);
+    2*|S|*|U| + 2 + |S|*(2*|S|*|U| + 2*|U| + 1);
+    2*|S|*|U| + 2 + (2*|S|*|S|*|U| + 2*|S|*|U| + |S|);
+    2*|S|*|S|*|U| + 4*|S|*|U| + |S| + 2;
+  }
+  3*|S|*|S|*|U|*|U| + 2*|S|*|U|*|U|*|U| + 2*|S|*|S|*|U| + 4*|S|*|U|*|U| + 4*|S|*|U| + |U|*|U| + |S| + 4*|U| + 2
 }
 
 lemma aux_lemma_1(U: set<int>, S: set<set<int>>, k: nat, s: set<int>, s': set<int>)
